mostly wokring???

Cslib/Computability/LambdaCalculus/LocallyNameless/Untyped/FullBetaConfluence.lean
@@ -153,83 +153,46 @@ lemma para_open_out (L : Finset Var) (mem : ∀ x, x ∉ L → (M ^ fvar x) ⭢�
   rw [subst_intro x M' _ q3 (para_lc_l para), subst_intro x N' _ q2 (para_lc_r para)]
   exact para_subst x (mem x q1) para
 
--- TODO: the Takahashi translation would be a much nicer and shorter proof, but I had difficultly
--- writing it for locally nameless terms.
+@[simp]
+def takahashi : Term Var → Term Var
+| bvar x => bvar x
+| fvar i => fvar i
+| abs M => abs M.takahashi
+| app (abs N) M => N.takahashi ^ M.takahashi
+| app L R => app L.takahashi R.takahashi
 
--- adapted from https://github.com/ElifUskuplu/Stlc_deBruijn/blob/main/Stlc/confluence.lean
-/-- Parallel reduction has the diamond property. -/
-theorem para_diamond : Diamond (@Parallel Var) := by
-  intros t t1 t2 tpt1
-  revert t2
-  induction tpt1 <;> intros t2 tpt2
-  case fvar x => exact ⟨t2, by aesop⟩
-  case abs s1 s2' xs mem ih => 
-    cases tpt2
-    case abs t2' xs' mem' =>
-      have ⟨x, qx⟩ := fresh_exists (xs ∪ xs' ∪ t2'.fv ∪ s2'.fv)
-      simp only [Finset.union_assoc, Finset.mem_union, not_or] at qx
-      have ⟨q1, q2, q3, q4⟩ := qx
-      have ⟨t', qt'_l, qt'_r⟩ := ih x q1 (mem' _ q2)
-      exists abs (t' ^* x)
-      constructor 
-      <;> [let z := s2'; let z := t2']
-      <;> apply Parallel.abs ((z ^ fvar x).fv ∪ t'.fv ∪ {x})
-      <;> intros y qy <;> simp only [open', close]
-      <;> [rw [←open_close x _ 0 q4]; rw [←open_close x _ 0 q3]] 
-      <;> refine para_open_close x y 0 ?_ qy <;> [exact qt'_l; exact qt'_r]
-  case beta s1 s1' s2 s2' xs mem ps ih1 ih2 => 
-    cases tpt2
-    case app u2 u2' s1pu2 s2pu2' => 
-      cases s1pu2
-      case abs s1'' xs' mem' =>
-        have ⟨x, qx⟩ := fresh_exists (xs ∪ xs' ∪ s1''.fv ∪ s1'.fv)
-        simp only [Finset.union_assoc, Finset.mem_union, not_or] at qx
-        obtain ⟨q1, q2, q3, q4⟩ := qx
-        have ⟨t', qt'_l, qt'_r⟩ := ih2 s2pu2'
-        have ⟨t'', qt''_l, qt''_r⟩ := @ih1 x q1 _ (mem' _ q2)
-        exists (t'' ^* x) ^ t'
-        constructor
-        · rw [subst_intro x s2' _ q4 (para_lc_l qt'_l), 
-              subst_intro x t' _ (close_var_not_fvar x t'') (para_lc_r qt'_l)]
-          simp only [open', close]
-          rw [close_open _ _ _ (para_lc_r qt''_l)]
-          exact para_subst x qt''_l qt'_l
-        · refine Parallel.beta ((s1'' ^ fvar x).fv ∪ t''.fv ∪ {x}) ?_ (by aesop)
-          intros y qy
-          rw [←open_close x s1'' 0 (by aesop)]
-          apply para_open_close <;> aesop
-    case beta u1' u2' xs' mem' s2pu2' => 
-      have ⟨x, qx⟩ := fresh_exists (xs ∪ xs' ∪ u1'.fv ∪ s1'.fv ∪ s2'.fv ∪ u2'.fv)
-      simp only [Finset.union_assoc, Finset.mem_union, not_or] at qx
-      have ⟨q1, q2, q3, q4, q5, q6⟩ := qx
-      have ⟨t', qt'_l, qt'_r⟩ := ih2 s2pu2'
-      have ⟨t'', qt''_l, qt''_r⟩ := @ih1 x q1 _ (mem' _ q2)
-      refine ⟨t'' [x := t'], ?_⟩
-      have : _ ∧ _ := ⟨para_subst x qt''_l qt'_l, para_subst x qt''_r qt'_r⟩
-      rw [subst_intro x u2' u1' _ (para_lc_l qt'_r), subst_intro x s2' s1' _ (para_lc_l qt'_l)]
-      all_goals aesop
-  case app s1 s1' s2 s2' s1ps1' _ ih1 ih2  =>
-    cases tpt2
-    case app u1 u2' s1 s2 =>
-      have ⟨l, _, _⟩ := ih1 s1
-      have ⟨r, _, _⟩ := ih2 s2
-      exact ⟨app l r, by aesop⟩
-    case beta t1' u1' u2' xs mem s2pu2' => 
-      cases s1ps1'
-      case abs s1'' xs' mem' =>
-        have ⟨x, qx⟩ := fresh_exists (xs ∪ xs' ∪ s1''.fv ∪ u1'.fv)
-        simp only [Finset.union_assoc, Finset.mem_union, not_or] at qx
-        obtain ⟨q1, q2, q3, q4⟩ := qx
-        have ⟨t', qt'_l, qt'_r⟩ := ih2 s2pu2'
-        have ⟨t'', qt''_l, qt''_r⟩ := @ih1 (abs u1') (Parallel.abs xs mem)
-        cases qt''_l
-        next w1 xs'' mem'' =>
-        cases qt''_r
-        case abs xs''' mem''' =>
-          exists w1 ^ t'
-          constructor
-          · aesop (config := {enableSimp := false})
-          · exact para_open_out xs''' mem''' qt'_r
+-- TODO: not sure this is true...
+theorem takahashi_openRec {M : Term Var} : M⟦k ↝ fvar x⟧.takahashi = M.takahashi⟦k ↝ fvar x⟧ := by
+  revert k x
+  induction M using takahashi.induct
+  case case4 l r ih_l ih_r => 
+    intros k x
+    sorry
+  case case5 l _ _ _ _ => induction l <;> aesop
+  all_goals aesop
+
+--@[simp]
+--theorem takahashi_open {M : Term Var} : (M ^ fvar x).takahashi = M.takahashi ^ fvar x := by
+--  exact takahashi_openRec
+
+theorem takahashi_triangle (M N : Term Var) (para : M ⭢ₚ N) : N ⭢ₚ M.takahashi := by
+  induction para
+  case fvar => aesop
+  case abs L q w => 
+    refine Parallel.abs L ?_
+    sorry
+  case beta L _ _ _ np => 
+    refine para_open_out L ?_ np
+    sorry
+  case app L' _ _ _ L_L' _ Lt Rt =>
+    induction L'
+    case abs =>
+      cases L_L'
+      cases Lt
+      next xs _ => exact Parallel.beta xs (by aesop) Rt
+    all_goals constructor <;> aesop
+
+theorem para_diamond : Diamond (@Parallel Var) := triangle_diamond takahashi_triangle
 
 /-- Parallel reduction is confluent. -/
 theorem para_confluence : Confluence (@Parallel Var) := 
